Update interop to match Low.GCMencrypt

src/arch/x64/interop/AESEncryptBlock.fsti
@@ -39,9 +39,14 @@ let keys_match (key:Ghost.erased (aes_key_LE AES_128)) (keys_b:B.buffer UInt8.t 
 open FStar.Mul
 
 // TODO: Complete with your pre- and post-conditions
-let pre_cond (h:HS.mem) (output_b:b8) (input_b:b8) (key:Ghost.erased (aes_key_LE AES_128)) (keys_b:b8) = live h output_b /\ live h input_b /\ live h keys_b /\ locs_disjoint [output_b;input_b;keys_b] /\ length output_b % 16 == 0 /\ length input_b % 16 == 0 /\ length keys_b % 16 == 0 /\ B.length keys_b == (nr AES_128 + 1) * 16 /\
-  keys_match key keys_b h
-  /\ B.length output_b >= 1 /\ B.length input_b >= 1
+let pre_cond (h:HS.mem) (output_b:b8) (input_b:b8) (key:Ghost.erased (aes_key_LE AES_128)) (keys_b:b8) = live h output_b /\ live h input_b /\ live h keys_b /\ length output_b % 16 == 0 /\ length input_b % 16 == 0 /\ length keys_b % 16 == 0 /\
+    disjoint_or_eq input_b output_b /\
+    disjoint keys_b input_b /\
+    disjoint keys_b output_b /\
+  B.length keys_b == (nr AES_128 + 1) * 16 /\
+    keys_match key keys_b h
+    /\ B.length output_b >= 1 /\ B.length input_b >= 1
+  
 
 
 let post_cond (h0:HS.mem) (h1:HS.mem) (output_b:b8) (input_b:b8) (key:Ghost.erased (aes_key_LE AES_128)) (keys_b:b8) = 
