SConscript
@@ -102,6 +102,7 @@ verify_options = {
 #  'src/arch/x64/X64.Bytes_Semantics_i.fst': None,
   'tools/Vale/test/vale-debug.vad': None,
   'tools/Vale/test/tactics1.vaf': None,
+  'src/crypto/aes/x64/Low.GCMencrypt.fst': None,
   'src/arch/x64/interop/*.fst': None,
   'src/arch/x64/interop/*.fsti': None,
   'src/arch/x64/interop/*.vaf': None,
